Core/Metatheory/GlobalWf.lean
@@ -1,0 +1,50 @@
+import LeanSubst
+import Core.Term
+import Core.Reduction
+import Core.Typing
+
+import Core.Metatheory.Substitution
+import Core.Metatheory.Rename
+import Core.Global
+
+
+theorem GlobalWf.weaken_type :
+  ⊢ G ->
+  GlobalWf G e ->
+  G&[], [] ⊢ t : T ->
+  (e :: G)&[], [] ⊢ t : T := by
+intro wf wfe j
+sorry
+
+
+theorem GlobalWf.weaken_kind e :
+  ⊢ G ->
+  GlobalWf G e ->
+  G&[] ⊢ T : K ->
+  (e :: G)&[] ⊢ T : K := by
+intro wf wfe j
+sorry
+
+
+
+theorem wf_lookup_kind_sound :
+  ⊢ G ->
+  lookup_type G x = some T ->
+  G&[] ⊢ T : .base b := by
+intro wf h
+-- generalize lkdef : lookup_type G x = lk at *
+induction wf generalizing x T
+case _ => simp [lookup_type, lookup, default] at *
+case _ G g gwf wf ih =>
+  replace ih := @ih x T
+  sorry
+
+
+theorem wf_lookup_type_sound :
+  ⊢ G ->
+  lookup_type G x = some T ->
+  G&Δ, Γ ⊢ g#x : T := by
+ intro wf h
+ constructor; assumption;
+ sorry
+ sorry
