Core/Metatheory/Preservation.lean
@@ -163,54 +163,256 @@ apply lem t' r
 theorem instance_type_preservation :
   ⊢ G ->
   G&Δ, Γ ⊢ g#x : T ->
-  instances x G = is ->
+  is = instances x G ->
   ∀ t ∈ is, G&Δ, Γ ⊢ t : T := by
 intro wf j h t t_in_is
 sorry
 
+theorem lookup_defn_type_sound :
+  ⊢ G ->
+  lookup_defn G x = .some t ->
+  G&Δ,Γ ⊢ g#x : T ->
+  G&Δ,Γ ⊢ t : T := by
+intro wf h1 h2
+sorry
+
+theorem Typing.foldr_preservation :
+  G&Δ ⊢ T : K ->
+  (∀ t ∈ is, G&Δ, Γ ⊢ t : T) ->
+  G&Δ, Γ ⊢ List.foldr (·`+·) `0 is : T := by
+intro j h
+induction is <;> simp at *
+constructor; assumption
+case _ hd tl ih =>
+  apply Typing.choice
+  apply j
+  apply h.1
+  apply ih h.2
+
+
+theorem preservation_prefix_match {p s t : Term} :
+  G&Δ,Γ ⊢ p : A ->
+  G&Δ,Γ ⊢ s : R ->
+  G&Δ,Γ ⊢ t : B ->
+  StableTypeMatch Δ A R ->
+  PrefixTypeMatch Δ A B T ->
+  some ξ = prefix_equal sp sp' ->
+  some (x, sp) = p.spine ->
+  some (x, sp') = s.spine ->
+  G&Δ,Γ ⊢ t.apply ξ : T
+:= by
+intro j1 j2 j3 j4 j5 j6 j7 j8
+induction s using Term.spine.induct generalizing x sp sp'
+case _ =>
+  simp [Term.spine] at j8; rcases j8 with ⟨j8, j9⟩
+  cases j8; cases j9
+  induction p using Term.spine.induct
+  case _ =>
+    simp [Term.spine] at j7; rcases j7 with ⟨j8, j9⟩
+    cases j8; cases j9
+    simp [prefix_equal] at j6; cases j6
+    simp [Term.apply]
+    sorry
+  simp [Term.spine] at j7; symm at j7
+  rw[Option.bind_eq_some_iff] at j7; rcases j7 with ⟨_, j7, j8⟩
+  sorry
+  sorry
+  sorry
+  sorry
+
+sorry
+sorry
+sorry
+sorry
+
+
 theorem preservation_lemma :
-  Δ = [] -> Γ = [] ->
+  ⊢ G ->
   G&Δ, Γ ⊢ t : T ->
   G ⊢ t ~> t' ->
   G&Δ, Γ ⊢ t' : T  := by
-intro e1 e2 j h
+intro wf j h
 induction j generalizing t' <;> simp at *
-case var h' _ => rw[e2] at h'; simp at h'
-all_goals (cases e1; cases e2)
+case var h' _ =>
+  cases h
+  case _ h _ => simp [Term.spine] at h
+  case _ h => simp [Term.spine] at h
 all_goals (try simp at *)
-case global => sorry
-  -- cases h; simp at *;
-  -- case _ h _ _ _ =>
-  -- cases h
-  -- sorry
+case global =>
+  cases h
+  case _ h _ =>
+    simp [Term.spine] at h; rcases h with ⟨e1, e2⟩; cases e1; cases e2;
+    simp [Term.apply] at *
+    case _ x A Δ K Γ h1 h2 _ tl _ _ _ _ is _ _ e =>
+    cases e
+    have lem : G&Δ, Γ ⊢ g#x : A := by constructor; apply h1; apply h2
+    replace lem := instance_type_preservation wf lem is
+    cases is; case _ e =>
+    cases e
+    apply Typing.foldr_preservation
+    apply h2
+    apply lem
+  case _ h =>
+    simp [Term.spine] at h; rcases h with ⟨e1, e2⟩; cases e1; cases e2;
+    simp [Term.apply] at *
+    apply lookup_defn_type_sound wf; assumption; constructor; assumption; assumption
+
 case mtch =>
-  sorry
+  cases h
+  case data_match pats _ j1 vhv j2 h1 h2 h3 h4 h5 _ _ _ _ x _ _ i patshapes' patshapes _ h6 h7 h8 h9 =>
+    apply preservation_prefix_match
+    apply (h2 i)
+    apply j1
+    apply h4 i
+    apply h3 i
+    apply h5 i
+    apply h7
+    · have lem : some ((patshapes i).fst, (patshapes i).snd) = (pats i).spine := by
+
+           sorry
+
+      have lem := Vec.indexOf_correct (v := Vec.map (λ x => x.1) patshapes) (i := i) (x := x) h6
+      sorry
+    apply h8
+
+  case data_match_default =>  assumption
+
+  case match_congr ih _ _ _ _ h =>
+    constructor
+    apply ih h
+    assumption
+    assumption
+    assumption
+    assumption
+    assumption
+    assumption
+    assumption
+
+  case match_absorb =>
+    -- need to show T is of base type
+    sorry
+  case match_map h ih =>
+    cases h
+    apply Typing.choice
+    sorry -- need to show T is of base type
+    · apply Typing.mtch; assumption; assumption; assumption; assumption; assumption; assumption; assumption; assumption
+    · apply Typing.mtch; assumption; assumption; assumption; assumption; assumption; assumption; assumption; assumption
+    sorry
+  all_goals (try case _ h => simp [Term.spine] at h)
+  all_goals (try case _ h _ => simp [Term.spine] at h)
+
 case guard =>
   cases h
-  case guard_matched => sorry
-  case guard_missed => sorry
+  case guard_matched h1 h2 h3 h4 h5 h6 h7 _ _ _ _ _ _ _ h8 h9 h10 =>
+    apply preservation_prefix_match
+    apply h1
+    apply h2
+    apply h3
+    apply h6
+    apply h7
+    apply h8
+    apply h9
+    apply h10
+
+  case guard_missed =>
+    sorry -- need to show T is of base type
+  case guard_congr ih _ _ h =>
+    constructor; assumption; apply ih h; assumption; assumption; assumption; assumption; assumption
+  case guard_absorb =>
+    sorry  -- need to show T is of base type
+  case guard_map h _ =>
+    cases h
+    apply Typing.choice
+    sorry -- T is of base type
+    · constructor; assumption; assumption; assumption; assumption; assumption; assumption; assumption
+    · constructor; assumption; assumption; assumption; assumption; assumption; assumption; assumption
+    sorry
   all_goals (try case _ h => simp [Term.spine] at h)
   all_goals (try case _ h _ => simp [Term.spine] at h)
   all_goals (try case _ h _ _ => simp at h)
-  · sorry
-  · sorry
-  · constructor
+
+case app b _ f _ a j1 j2 j3 _ _ =>
+  cases h
+  all_goals (try case _ h => simp [Term.spine] at h)
+  all_goals (try case _ h _ => simp at h)
+  all_goals (try case _ h _ _ => simp at h)
+  case beta =>
+    cases j2; apply Typing.beta wf; assumption; assumption
+  case inst => sorry
+  case defn => sorry
+  case ctor2_congr1 ih _ _ _ h =>
+    apply Typing.app
+    assumption
+    apply ih h
+    assumption
+  case ctor2_congr2 ih _ _ h =>
+    apply Typing.app; assumption; assumption; apply ih h
+  case ctor2_absorb1 => cases j2; case _ j2 => cases j2; constructor; assumption
+  case ctor2_absorb2 => sorry
+  case ctor2_map1 =>
+    cases j2; case _ j2 _ _ =>
+    cases j2
+    apply Typing.choice
+    assumption
+    · constructor; assumption; assumption; assumption
+    · constructor; assumption; assumption; assumption
+  case ctor2_map2 =>
+    cases j3
+    apply Typing.choice
     sorry
-    sorry
-    sorry
+    · constructor; assumption; assumption; assumption
+    · constructor; assumption; assumption; assumption
     sorry
 
-case app => sorry
-case appt => sorry
+case appt f _ _ a _ j1 j2 _ _ =>
+  cases h
+  all_goals (try case _ h => simp [Term.spine] at h)
+  all_goals (try case _ h _ => simp at h)
+  all_goals (try case _ h _ _ => simp at h)
+  case betat Δ Γ K P _ e A b _ =>
+    cases j1; case _ j1 =>
+    rw[e];
+    have lem := @Typing.beta_type G K Δ (Γ.map (λ x => x[+1])) b P a wf j1 j2
+    simp at lem
+    have lem2 : List.map ((λ x => x[su a::+0]) ∘ (λ x => x[+1])) Γ = Γ := by
+      generalize fdef : (λ x => x[su a::+0]) ∘ (λ x => x[+1]) = f at *
+      simp [Function.comp_def] at fdef
+      rw[<-fdef]; simp
+    rw[lem2] at lem
+    assumption
+  case inst => sorry
+  case defn => sorry
+  case ctor1_congr ih _ h =>
+    apply Typing.appt
+    apply ih h
+    assumption
+    assumption
+  case ctor1_absorb =>
+    cases j1; case _ j1 =>
+    cases j1; case _ e _ _ j1 =>
+    have lem := Kinding.beta j1 j2
+    rw[e]; constructor; assumption
+  case ctor1_map =>
+    cases j1
+    case _ j _ _ =>
+      cases j; case _ e _ _ _ _ _ _ _ _ _ j1 =>
+      rw[e]
+      apply Typing.choice
+      apply Kinding.beta j1 j2
+      · apply Typing.appt; assumption; assumption; simp
+      · apply Typing.appt; assumption; assumption; simp
+
 case lam =>
-  cases h;
+  cases h
   case _ h _ => cases h
   case _ h => simp [Term.spine] at h
 case lamt =>
-  cases h;
+  cases h
   case _ h _ => cases h
   case _ h => simp [Term.spine] at h
-  all_goals (case _ h _ => simp at h)
+  case _ h _ => simp at h
+  all_goals (case _ h _ _ => simp at h)
+
 case cast tj cj _ ih =>
   cases h
   all_goals (try case _ h => simp [Term.spine] at h)
@@ -260,59 +462,119 @@ case seq =>
   all_goals (try case _ h => simp [Term.spine] at h)
   all_goals (try case _ h _ => simp [Term.spine] at h)
   all_goals (try case _ h _ _ => simp at h)
-  sorry
-  sorry
-  sorry
-  sorry
-  sorry
-  sorry
-  sorry
-case appc => sorry
-case arrowc => sorry
-case fst => sorry
-case snd => sorry
-case allc =>
+  case seq j1 _ j2 _  => cases j1; cases j2; constructor; assumption
+  case ctor2_congr1 ih _ _ _ h =>
+    constructor
+    apply ih h
+    assumption
+  case ctor2_congr2 ih _ _ h =>
+    constructor
+    assumption
+    apply ih h
+  case ctor2_absorb1 j1 _ _ j2 _ =>
+    cases j2; case _ j2 =>
+    cases j2;
+    -- need some nice properties from wf contexts
+    sorry
+  case ctor2_absorb2 =>
+
+    sorry
+  case ctor2_map1 j1 _ _ _ _ _ j2 _  =>
+    cases j2; case _ j2 _ _ =>
+    cases j2
+    apply Typing.choice
+    constructor;
+    · assumption
+    · sorry
+    constructor
+    assumption
+    assumption
+    constructor; assumption; assumption
+
+  case ctor2_map2 =>
+    sorry
+case appc Δ Γ _ K1 K2 A B _ C D _ _ _ _ =>
   cases h
   all_goals (try case _ h => simp [Term.spine] at h)
   all_goals (try case _ h _ => simp [Term.spine] at h)
-  all_goals (try case _ h _ _ => simp [Term.spine] at h)
-  case _ h => cases h; case _ h => constructor; constructor; assumption
-  case _ h _ =>
-    simp at h
-    constructor; simp;
-    sorry -- where did my induction hypothesis go?
-    sorry
-  case _ h =>
-    cases h; case _ h =>
-    cases h;
-    constructor; constructor; sorry; sorry
-  case _ h =>
-    cases h
-    constructor
-    constructor;
-    sorry;
-    sorry
-    constructor; simp; assumption
-    constructor; simp; assumption
+  all_goals (try case _ h _ _ => simp at h)
+  case appc j1 _ j2 _ =>
+    cases j1; cases j2
+    apply @Typing.refl G Δ (A • C) K2 Γ
+    constructor; assumption; assumption
+
+  case ctor2_congr1 => sorry
+  case ctor2_congr2 => sorry
+  case ctor2_absorb1 => sorry
+  case ctor2_absorb2 => sorry
+  case ctor2_map1 => sorry
+  case ctor2_map2 => sorry
+
+case arrowc =>
+  cases h
+  all_goals (try case _ h => simp [Term.spine] at h)
+  all_goals (try case _ h _ => simp [Term.spine] at h)
+  all_goals (try case _ h _ _ => simp at h)
+  case arrowc => sorry
+
+  case ctor2_congr1 => sorry
+  case ctor2_congr2 => sorry
+  case ctor2_absorb1 => sorry
+  case ctor2_absorb2 => sorry
+  case ctor2_map1 => sorry
+  case ctor2_map2 => sorry
+
+case fst =>
+  cases h
+  all_goals (try case _ h => simp [Term.spine] at h)
+  all_goals (try case _ h _ => simp [Term.spine] at h)
+  all_goals (try case _ h _ _ => simp at h)
+  case fst => sorry
+  case ctor1_congr => sorry
+  case ctor1_absorb => sorry
+  case ctor1_map => sorry
+
+case snd =>
+  cases h
+  all_goals (try case _ h => simp [Term.spine] at h)
+  all_goals (try case _ h _ => simp [Term.spine] at h)
+  all_goals (try case _ h _ _ => simp at h)
+  case snd => sorry
+  case ctor1_congr => sorry
+  case ctor1_absorb => sorry
+  case ctor1_map => sorry
+
+case allc K Δ _ _ A B Γ j _ =>
+  cases h
+  all_goals (try case _ h => simp [Term.spine] at h)
+  all_goals (try case _ h _ => simp [Term.spine] at h)
+  all_goals (try case _ h _ _ => simp at h)
+  case allc B _ =>
+    cases j; case _ b j _ =>
+    apply @Typing.refl G Δ (∀[K]A) ★ Γ (Kinding.all j)
+  case tbind_congr => sorry
+  case tbind_absorb => sorry
+  case tbind_map => sorry
 
 case apptc =>
   cases h
   all_goals (try case _ h => simp [Term.spine] at h)
   all_goals (try case _ h _ => simp [Term.spine] at h)
   all_goals (try case _ h _ _ => simp at h)
-  case _ e1 e2 _ _ _ h1 _ h2 _ =>
+  case apptc e1 e2 _ _ _ h1 _ h2 _ =>
     cases h1; cases h2
-    rw[<-e1] at e2; rw[e2]; rw[e1]
+    rw[<-e1] at e2; subst e2; subst e1
     constructor; case _ j1 _ j2 _ =>
     cases j1; case _ j1 =>
     have lem := Kinding.beta j1 j2
     sorry
-  case _ => sorry
-  case _ => sorry
-  case _ => sorry
-  case _ => sorry
-  case _ => sorry
-  case _ => sorry
+
+  case ctor2_congr1 => sorry
+  case ctor2_congr2 => sorry
+  case ctor2_absorb1 => sorry
+  case ctor2_absorb2 => sorry
+  case ctor2_map1 => sorry
+  case ctor2_map2 => sorry
 
 case zero =>
   cases h;
@@ -331,9 +593,3 @@ case choice =>
     replace ih := ih r
     apply Typing.choice; assumption; assumption; assumption
   all_goals (case _ h _ _ => simp at h)
-
-
-theorem preservation :
-  G&[], [] ⊢ t : T ->
-  G ⊢ t ~> t' ->
-  G&[], [] ⊢ t' : T  := by intro j r; apply preservation_lemma rfl rfl j r
